Utlc/LemmasEvaluation.v
@@ -15,7 +15,7 @@ Local Ltac crush :=
   try discriminate;
   eauto.
 
-Section SubstEval.
+Section EvaluationContexts.
 
   Lemma pctx_app_sub' C :
     ∀ (ζ: Sub UTm) t,
@@ -29,6 +29,16 @@ Section SubstEval.
       pctx_app t[ζ ↑⋆ depthPCtx C] C[ζ].
   Proof. induction C; crush. Qed.
 
+  Lemma pctx_cat_app (t : UTm) (C₁ C₂ : PCtx) :
+    pctx_app t (pctx_cat C₁ C₂) = pctx_app (pctx_app t C₁) C₂.
+  Proof.
+    induction C₂; crush.
+  Qed.
+
+  Lemma ectx_cat (C₁ C₂: PCtx) :
+    ECtx C₁ → ECtx C₂ → ECtx (pctx_cat C₁ C₂).
+  Proof. induction C₂; crush. Qed.
+
   Lemma value_sub t (v: Value t) :
     ∀ (ζ: Sub UTm), Value t[ζ].
   Proof. induction t; crush. Qed.
@@ -37,6 +47,76 @@ Section SubstEval.
   Lemma ectx_sub C (ectx_C: ECtx C) :
     ∀ (ζ: Sub UTm), ECtx C[ζ].
   Proof. induction C; crush. Qed.
+  Hint Resolve ectx_sub.
+
+End EvaluationContexts.
+
+(* The following doesn't hold here: C[wrong] evaluates to wrong in single step *)
+(* Lemma eval_ctx {C t t'}  : t --> t' -> ECtx C -> pctx_app t C --> pctx_app t' C. *)
+(* Proof. *)
+(*   induction 1. *)
+(*   rewrite <- ?pctx_cat_app in *. *)
+(*   eauto using ectx_cat with eval. *)
+(* Qed. *)
+
+Section Values.
+
+  Lemma value_pctx_inversion {C} (eC: ECtx C) :
+    ∀ t, Value (pctx_app t C) → Value t.
+  Proof. induction C; cbn in *; intuition. Qed.
+
+  Lemma ectx_wrong_not_value {C} : ECtx C -> ¬ (Value (pctx_app wrong C)).
+  Proof.
+    intros ec val.
+    apply value_pctx_inversion in val; crush.
+  Qed.
+
+  Lemma values_are_eval₀_normal {t t'} :
+    Value t → t -->₀ t' → False.
+  Proof. inversion 2; crush. Qed.
+
+  Lemma values_are_normal {t : UTm} : Value t → normal t.
+  Proof.
+    intros vt; induction 1 as [? ? ? r'|?];
+      apply value_pctx_inversion in vt;
+      eauto using values_are_eval₀_normal.
+  Qed.
+  Global Arguments values_are_normal {_} _ {_} _.
+
+End Values.
+
+Section Termination.
+
+  Lemma TerminatingI' (t: UTm) (vt: Value t) :
+    ∀ t', t --> t' → t'⇓.
+  Proof. intros t' r; elim (values_are_normal vt r). Qed.
+
+  Lemma TerminatingIV' (t: UTm) (vt: Value t) :
+    ∀ t' n, t --> t' → t'⇓_n.
+  Proof. intros t' n r; elim (values_are_normal vt r). Qed.
+
+  Lemma values_terminate (t: UTm) (vt: Value t) :
+    t ⇓.
+  Proof. constructor; eauto using TerminatingI'. Qed.
+
+  Lemma values_terminateN (t: UTm) (vt: Value t) :
+    ∀ n, t ⇓_ n.
+  Proof. constructor; eauto. Qed.
+
+  Lemma TerminatingDN (t: UTm) n (m: t ⇓_ (S n)) :
+    ∀ t' : UTm, t --> t' → t'⇓_n.
+  Proof. depind m; eauto using TerminatingIV'. Qed.
+
+  Lemma TerminatingN_Terminating {t : UTm} {n} : t ⇓_ n -> t ⇓.
+  Proof. induction 1;
+    eauto using Terminating, values_terminate with eval.
+  Qed.
+
+End Termination.
+
+Section SubstEval.
+
+  Hint Resolve value_sub.
   Hint Resolve ectx_sub.
 
   Lemma eval₀_closed_under_substitution {t1 t2} (r: t1 -->₀ t2) :
@@ -53,68 +133,10 @@ Section SubstEval.
   Lemma eval_closed_under_substitution {t1 t2} (r: t1 --> t2) (ζ: Sub UTm) :
     t1[ζ] --> t2[ζ].
   Proof.
-    induction r as [C t₁' t₂' e|C]; rewrite -> ?pctx_app_sub.
-    - constructor; eauto using eval₀_closed_under_substitution.
-    - constructor; induction C; crush.
+    induction r as [C t₁' t₂' e|C];
+    rewrite -> ?pctx_app_sub; constructor;
+      auto using eval₀_closed_under_substitution.
+    destruct C; crush.
   Qed.
 
 End SubstEval.
-
-Lemma ectx_cat (C₁ C₂: PCtx) :
-  ECtx C₁ → ECtx C₂ → ECtx (pctx_cat C₁ C₂).
-Proof.
-  induction C₂; simpl; intros; destruct_conjs; auto.
-Qed.
-
-Lemma pctx_cat_app (t : UTm) (C₁ C₂ : PCtx) :
-  pctx_app t (pctx_cat C₁ C₂) = pctx_app (pctx_app t C₁) C₂.
-Proof.
-  induction C₂; crush.
-Qed.
-
-(* The following doesn't hold here: C[wrong] evaluates to wrong in single step *)
-(* Lemma eval_ctx {C t t'}  : t --> t' -> ECtx C -> pctx_app t C --> pctx_app t' C. *)
-(* Proof. *)
-(*   induction 1. *)
-(*   rewrite <- ?pctx_cat_app in *. *)
-(*   eauto using ectx_cat with eval. *)
-(* Qed. *)
-
-Lemma ectx_wrong_not_value {C} : ECtx C -> not (Value (pctx_app wrong C)).
-Proof.
-  intros ec val.
-  induction C; crush.
-Qed.
-
-Definition normal' (t : UTm) := ∀ t', ¬ (t --> t').
-Lemma values_are_normal' {t : UTm} : Value t -> normal' t.
-Proof.
-  intros vt t' r; revert vt.
-  induction r as [C ? ? r'|C]; crush.
-  - induction C; crush.
-    inversion r'; crush.
-  - now apply ectx_wrong_not_value in vt.
-Qed.
-
-Lemma values_are_normal {t : UTm} : Value t -> normal t.
-Proof.
-  generalize @values_are_normal'.
-  unfold normal, normal', not.
-  intros ? ? (); eauto.
-Qed.
-
-Lemma TerminatingDN (t: UTm) n (m: t ⇓_ (S n)) :
-  ∀ t', t --> t' → TerminatingN t' n.
-Proof. 
-  depind m; intros t' e'; eauto using values_are_normal.
-  exfalso.
-  refine (values_are_normal H _); exists t'; auto.
-Qed.
-
-
-Lemma TerminatingN_Terminating {t : UTm} {n} : t ⇓_ n -> t ⇓.
-Proof.
-  induction 1; constructor; try assumption.
-  intros t' e'. exfalso. refine (values_are_normal H _).
-  exists t'. auto.
-Qed.
